Make various surface-level cleanups (indentation etc)
Remove occasional unused theorems too.

examples/computability/turingMachines/turing_machineScript.sml
@@ -125,183 +125,67 @@ val _ = overload_on("RUN",``FUNPOW UPDATE_TAPE``);
 
 
 val DECODE_def = tDefine "DECODE" `
-(DECODE 0 = []) ∧
-(DECODE n = if (ODD n)
-            then [O] ++ (DECODE ((n-1) DIV 2))
-            else [Z] ++ (DECODE (n DIV 2)))`
-(WF_REL_TAC `$<` >> rw[] >> intLib.ARITH_TAC)
+  (DECODE 0 = []) ∧
+  (DECODE n = if (ODD n) then [O] ++ (DECODE ((n-1) DIV 2))
+              else [Z] ++ (DECODE (n DIV 2)))`
+  (WF_REL_TAC `$<` >> rw[] >> intLib.ARITH_TAC)
 
 
-val ENCODE_def = Define `(ENCODE [] = 0) ∧
-(ENCODE (h::t) = case h of
+val ENCODE_def = Define `
+  (ENCODE [] = 0) ∧
+  (ENCODE (h::t) = case h of
                      Z => 0 + (2 * (ENCODE t))
                    | O => 1 + (2 * (ENCODE t))
                    | _ => 0)`;
-
-
-EVAL `` (DECODE (ENCODE [O;O;Z;O;Z;O;Z;O;O;O]) )``;
-
-EVAL `` ENCODE (DECODE 99999999999)``;
-
-EVAL ``ENCODE [O;Z;Z;Z;Z]``;
 
 (* Change TO simpler def of DECODE*)
 
 (* Lemmas for ENCODE/DECODE*)
 
-val SUC_CANCEL_lem = Q.store_thm(
-        "SUC_CANCEL_lem",
-`! n m. (SUC n = SUC m) ==> (m = n)`,
-Induct_on `n` >- fs[]
-          >> Induct_on `m`
->- fs[]
->- fs[]
-    );
-
-val DIV_3_lem = Q.store_thm(
-        "DIV_3_lem",
-    `∀ n.(n DIV 3 = 0) ==> (n<3) `,
-    Induct_on `n` >- fs[] >> strip_tac
-              >> `SUC 0 DIV 3 = 0` by fs[]
-              >> `SUC 1 DIV 3 = 0` by fs[]
-              >> Cases_on `n`
-              >- fs[]
-              >> Cases_on `n'`
-                >- fs[]
-                >> Cases_on `n`
-                  >- fs[]
-                  >> `n'>= 0` by fs[]
-                  >> `SUC (SUC (SUC (SUC n'))) >= 3` by fs[]
-                  >> `~(SUC (SUC (SUC (SUC n'))) < 3)` by fs[]
-                  >> fs[]
-                  >> `SUC (SUC (SUC (SUC n'))) = n' + 4` by fs[]
-                  >> `SUC (SUC (SUC n')) = n' + 3` by fs[]
-                  >> `n' + 3 DIV 3 ≠ 0` by fs[]
-                  >> `(n' + 4 DIV 3 = 0) <=> F` by fs[]
-                  >> rw[]
-                  >> `SUC (SUC (SUC (SUC n'))) DIV 3 <= n' + 4 DIV 3` by fs[]
-                  >> `(SUC (SUC (SUC (SUC n')))) DIV 3 = (n' + 4) DIV 3` by prove_tac[]
-                  >> `(n'+4) DIV 3 = 0` by fs[]
-                  >> `n'+4 = (n'+4)` by fs[]
-                  >> `n'>=0` by fs[]
-                  >> `4 <= n'+4` by fs[]
-                  >> `0<3` by fs[]
-                  >> `4 DIV 3 = 1` by fs[]
-                  >> `4 DIV 3 <= (n' +4) DIV 3` by metis_tac[DIV_LE_MONOTONE]
-                  >> `1 <=0` by fs[]
-                  >> fs[]
-    );
-
-
-(* Examples *)
-
-EVAL ``LENGTH (TL [h])``;
-
-
-EVAL ``2 MOD 3``;
-
-
-(*
-val ENCODE_DECODE_lem_Z = Q.store_thm(
-    "ENCODE_DECODE_lem1[simp]",
-    `!n. ENCODE_tern (2*(3**(LENGTH n)) + DECODE n) = Z::n`,
-    strip_tac >> completeInduct_on `LENGTH n` >> strip_tac
-    >> strip_tac >> Cases_on `LENGTH n` >- fs[] >> EVAL_TAC >>
-    >> strip_tac >> strip_tac
-    );
-*)
-
 val ENCODE_DECODE_thm = store_thm(
-    "ENCODE_DECODE_thm",
-    ``!n. ENCODE (DECODE n) = n``,
-    completeInduct_on `n` >> Cases_on `n` >- EVAL_TAC >> rw[DECODE_def] >- (rw[ENCODE_def]
-    >> `0<2` by fs[] >> `n' DIV 2 <= n'` by metis_tac[DIV_LESS_EQ]
-    >> `n' < SUC n'` by fs[] >> `n' DIV 2 < SUC n'` by fs[]
-    >> `ENCODE (DECODE (n' DIV 2)) = n' DIV 2` by fs[] >> rw[]
-    >> `~ODD n'` by metis_tac[ODD]
-    >> `EVEN n'` by metis_tac[EVEN_OR_ODD]
-    >> `n' MOD 2 =0` by metis_tac[EVEN_MOD2]
-    >> `2 * (n' DIV 2) = n'` by metis_tac[MULT_EQ_DIV]
-    >> rw[])
-    >> rw[ENCODE_def]
-    >> `EVEN (SUC n')` by metis_tac[EVEN_OR_ODD]
-    >> `(SUC n') MOD 2 =0` by metis_tac[EVEN_MOD2]
-    >> `2 * ((SUC n') DIV 2) = SUC n'` by fs[MULT_EQ_DIV]
- );
+  "ENCODE_DECODE_thm",
+  ``!n. ENCODE (DECODE n) = n``,
+  completeInduct_on `n` >> Cases_on `n` >- EVAL_TAC >> rw[DECODE_def]
+  >- (rw[ENCODE_def]
+      >> `0<2` by fs[] >> `n' DIV 2 <= n'` by metis_tac[DIV_LESS_EQ]
+      >> `n' < SUC n'` by fs[] >> `n' DIV 2 < SUC n'` by fs[]
+      >> `ENCODE (DECODE (n' DIV 2)) = n' DIV 2` by fs[] >> rw[]
+      >> `~ODD n'` by metis_tac[ODD]
+      >> `EVEN n'` by metis_tac[EVEN_OR_ODD]
+      >> `n' MOD 2 =0` by metis_tac[EVEN_MOD2]
+      >> `2 * (n' DIV 2) = n'` by metis_tac[MULT_EQ_DIV]
+      >> rw[])
+  >> rw[ENCODE_def]
+  >> `EVEN (SUC n')` by metis_tac[EVEN_OR_ODD]
+  >> `(SUC n') MOD 2 =0` by metis_tac[EVEN_MOD2]
+  >> `2 * ((SUC n') DIV 2) = SUC n'` by fs[MULT_EQ_DIV]);
 
 val DECODE_EMPTY_lem = Q.store_thm (
-        "DECODE_EMPTY_lem",
-`∀ n. (DECODE n = []) ==> (n=0)`,
-    Induct_on `n` >- EVAL_TAC >> fs[] >> rw[DECODE_def]  );
+  "DECODE_EMPTY_lem",
+  `∀ n. (DECODE n = []) ==> (n=0)`,
+  Induct_on `n` >- EVAL_TAC >> fs[] >> rw[DECODE_def]  );
 
-(*
-Not a theorem
-
-val DECODE_ENCODE_thm = store_thm(
-    "DECODE_ENCODE_thm",
-    `!l. DECODE (ENCODE l) = l`,
-    completeInduct_on `ENCODE l` >> rpt  strip_tac >>  Cases_on `DECODE (ENCODE l)` >-
-        (`DECODE 0 = []` by fs[DECODE_def]
-      >> Cases_on `l` >- fs[] >> fs[] >> `ENCODE (h::t) = 0` by fs[DECODE_EMPTY_lem]
-      >> rw[])
-      >> rw[] >> Cases_on `h` >- ( rw[DECODE_def,ENCODE_def] )
-
-    );
-*)
-
-EVAL ``7 DIV 3``;
-
-val ENCODE_TM_TAPE_def = Define `ENCODE_TM_TAPE tm =
+val ENCODE_TM_TAPE_def = Define `
+  ENCODE_TM_TAPE tm =
        if tm.tape_h = Z then
-           ((ENCODE tm.tape_l) *,  (2 * (ENCODE tm.tape_r)))
+           (ENCODE tm.tape_l   *,   (2 * (ENCODE tm.tape_r)))
        else
-           ((ENCODE tm.tape_l) *, ( (2 * (ENCODE tm.tape_r)) + 1 ))`;
+           (ENCODE tm.tape_l   *,   (2 * (ENCODE tm.tape_r) + 1))
+`;
 
-val DECODE_TM_TAPE_def = Define `DECODE_TM_TAPE n =
+val DECODE_TM_TAPE_def = Define `
+  DECODE_TM_TAPE n =
        if EVEN (nsnd n) then
            (DECODE (nfst n), Z , DECODE ( (nsnd n) DIV 2))
        else
-           (DECODE (nfst n), O , DECODE ( ((nsnd n) - 1) DIV 2))`;
+           (DECODE (nfst n), O , DECODE ( (nsnd n - 1) DIV 2))`;
 
 (* Halted definition and TM examples *)
-
-
 val HALTED_def = Define `HALTED tm <=> (tm.state.n = 0)`;
 
 val st_def= Define`st n : state = <| n := n  |>`;
 val _ = add_numeral_form(#"s", SOME "st");
 
-
-(* EVAL ``(RUN 3
-   <| state := 0;
-      prog := FEMPTY |++ [((0,Z),(0,R)); ((0,O),(0,R)); ((1,O),(1,Wr0))] ;
-      tape_l := [];
-      tape_h := Z;
-      tape_r := [Z]
-     |>
-      [Z])``; *)
-
-
-(* unary addition machine *)
-                          (*
-EVAL ``(RUN 10
-   <| state := 0;
-        prog := FEMPTY |++ [((0,Z),(1,Wr1)); ((0,O),(0,R));
-                            ((1,Z),(2,L)); ((1,O),(1,R));
-                            ((2,O),(3,Wr0)) ] ;
-      tape_l := [];
-      tape_h := Z;
-      tape_r := [] |>
-      [O;O;O;Z;O;O])``;
-
-
-type_of ``(SET_TO_LIST (FDOM (<| state := 0;
-       prog := FEMPTY |++ [((0,Z),(0,R)); ((0,O),(1,Wr0)); ((1,Z),(1,R)); ((1,O),(2,Wr1)) ] ;
-       tape_l := [];
-       tape_h := Z;
-       tape_r := [Z] |>.prog)))
-       ``;
-*)
 
 (*
 
@@ -314,120 +198,41 @@ One can enumerate the Valid Turing Machines (by enumerating programs)
 
 *)
 
-val NUM_CELL_def = Define `(NUM_CELL Z = 0:num) ∧
+val NUM_CELL_def = Define `
+  (NUM_CELL Z = 0:num) ∧
   (NUM_CELL O = 1:num) `;
 
-val CELL_NUM_def = Define `(CELL_NUM 0n = Z) ∧
+val CELL_NUM_def = Define `
+  (CELL_NUM 0n = Z) ∧
   (CELL_NUM 1 = O) `;
 
-val ACT_TO_NUM_def = Define `(ACT_TO_NUM Wr0 = 0:num) ∧
+val ACT_TO_NUM_def = Define `
+  (ACT_TO_NUM Wr0 = 0:num) ∧
   (ACT_TO_NUM Wr1 = 1:num) ∧
   (ACT_TO_NUM L   = 2:num) ∧
   (ACT_TO_NUM R   = 3:num) `;
 
-val NUM_TO_ACT_def = Define `(NUM_TO_ACT 0n = Wr0 ) ∧
+val NUM_TO_ACT_def = Define `
+  (NUM_TO_ACT 0n = Wr0 ) ∧
   (NUM_TO_ACT 1 = Wr1) ∧
   (NUM_TO_ACT 2 = L) ∧
   (NUM_TO_ACT 3 = R) `;
-
-EVAL ``ACT_TO_NUM (NUM_TO_ACT 2)``;
-
-
-(* Definition of a Turing complete function, not working atm *)
-
-(*
-val TURING_COMPLETE_def = Define `TURING_COMPLETE f = ∃ tm. ∀ n. ∃ t. DECODE_TM_TAPE (RUN t tm (ENCODE n)) = f `
-*)
-
-(*
-Previous idea, using enumeration over program set
-*)
-
-EVAL ``HD (ncons_inv 88)``;
-
-EVAL ``HD (TL (ncons_inv 88))``;
-
-EVAL `` ncons (HD (ncons_inv 88)) (HD (TL (ncons_inv 88)))``;
-
-(*
-Previous diea of enumerating programs
-
-val NCONS_INVERSE_def = Define `(ncons_inv 1 = []) ∧ (ncons_inv c = [nfst (c-1) ; nsnd (c-1)] )`;
-
-EVAL `` MIN_SET {1:num;2:num;3:num;5:num;10:num}``;
-
-val LEAST_IN_SET_def = Define `
-LEAST_IN_SET s = let nconsset = { ncons (STATE_TO_NUM (FST c)) (NUM_CELL (SND c)) | c IN s } in
-  ncons_inv (MIN_SET nconsset) `;
-
-val LEAST_SET_TO_LIST_def = Define `
-LEAST_SET_TO_LIST s =
-if FINITE s then
-  if s={} then []
-  else let k = (NUM_TO_STATE (HD (LEAST_IN_SET s)), CELL_NUM (HD (TL (LEAST_IN_SET s))))  in
-    k :: LEAST_SET_TO_LIST (s DELETE k)
-else ARB`;
-
-val tcons_def = Define `
-tcons a b tm = (ncons (STATE_TO_NUM a) (NUM_CELL b)) *,
-                                                     (ncons (STATE_TO_NUM (FST (FAPPLY tm.prog ((a),(b)) ))) (NUM_ACT (SND (FAPPLY tm.prog ((a),(b)) )))) + 1`;
-
-val tlist_of = Define `
-(tlist_of [] tm = 0) ∧
-(tlist_of (h::t) tm = ncons (tcons (FST h) (SND h) tm)  (tlist_of t tm))`;
-
-val TURING_MACHINE_P_ENCODING_def = Define `
-TURING_MACHINE_P_ENCODING tm = tlist_of (SET_TO_LIST (FDOM tm.prog)) tm`;
-
-val FULL_ENCODE_TM_with_P_def = Define `FULL_ENCODE_TM_with_P tm =
-nlist_of [TURING_MACHINE_P_ENCODING tm; STATE_TO_NUM tm.state ; DECODE_TM_TAPE tm] `;
-
-
-*)
-
-(*
-Idea is, for each instruction in the program, which is an (a,b,c,d)
-val tcons_def = Define `
-(tcons (a,b,c,d) = (ncons a (NUM_CELL b)) *, (ncons c (NUM_ACT d)) + 1)`;
-*)
 
 val STATE_TO_NUM_def = Define `STATE_TO_NUM a = a.n`;
 
 val NUM_TO_STATE_def = Define `NUM_TO_STATE n = <| n:=n |>`;
 
-
-EVAL ``STATE_TO_NUM (NUM_TO_STATE 10)``;
-
-val FULL_ENCODE_TM_def = Define `FULL_ENCODE_TM tm =
- STATE_TO_NUM tm.state *, ENCODE_TM_TAPE tm `;
+val FULL_ENCODE_TM_def = Define `
+  FULL_ENCODE_TM tm = STATE_TO_NUM tm.state *, ENCODE_TM_TAPE tm
+`;
 
 
-val FULL_DECODE_TM_def = Define `FULL_DECODE_TM n =
-<|state:=  NUM_TO_STATE (nfst n);  tape_l := FST (DECODE_TM_TAPE (nsnd n));
-tape_h := FST (SND (DECODE_TM_TAPE (nsnd n)));
-tape_r := SND (SND (DECODE_TM_TAPE (nsnd n)))|> `;
-
-
-
-
-
-(* EVAL and type checks *)
-
-(*
-num_step tm (takes tm as number and does step, purely arithmetic)
-*)
-
-EVAL ``FULL_ENCODE_TM <| state := 0;
-prog := FEMPTY |++ [((0,Z),(0,R)); ((0,Z),(1,Wr0)); ((1,Z),(1,R)); ((1,Z),(2,Wr0)) ] ;
-tape_l := [];
-tape_h := Z;
-tape_r := [Z;O;O] |>``;
-
-EVAL `` FULL_DECODE_TM 4185``;
-
-type_of ``recfn f 1``;
-
-
+val FULL_DECODE_TM_def = Define `
+  FULL_DECODE_TM n = <| state:=  NUM_TO_STATE (nfst n);
+                        tape_l := FST (DECODE_TM_TAPE (nsnd n));
+                        tape_h := FST (SND (DECODE_TM_TAPE (nsnd n)));
+                        tape_r := SND (SND (DECODE_TM_TAPE (nsnd n)))|>
+`;
 
 (* Perform action an move to state *)
 val UPDATE_ACT_S_TM_def = Define `UPDATE_ACT_S_TM s act tm =
@@ -451,88 +256,38 @@ val UPDATE_ACT_S_TM_def = Define `UPDATE_ACT_S_TM s act tm =
                tape_h := HD tm.tape_r;
                tape_r := TL tm.tape_r |>`;
 
-(* EVAL checks *)
-
-EVAL ``FULL_ENCODE_TM (UPDATE_ACT_S_TM 0 Wr1 <| state := 0;
-               prog := FEMPTY |++ [((0,Z),(0,R)); ((0,Z),(1,Wr0)); ((1,Z),(1,R)); ((1,Z),(2,Wr0)) ] ;
-               tape_l := [];
-               tape_h := Z;
-               tape_r := [Z;O;O] |>)``;
-
-
-
-EVAL `` 0 *, nsnd 10``;
-
 val ODD_DIV_2_lem = Q.store_thm ("ODD_DIV_2_lem",
-`∀ y. ODD y ==> (y DIV 2 = (y-1) DIV 2)`,
-Induct_on `y` >- EVAL_TAC >> rw[] >> `SUC y = y+1` by fs[] >> rw[] >>
-`~(ODD y)` by fs[ODD] >>
-`1 DIV 2 = 0` by EVAL_TAC >> `0<2` by fs[] >> `EVEN y` by metis_tac[EVEN_OR_ODD] >>
-`y MOD 2 = 0` by metis_tac[EVEN_MOD2] >>
-`(y+1) DIV 2 = (y DIV 2) + (1 DIV 2)` by fs[ADD_DIV_RWT] >> rw[]
-);
+  `∀ y. ODD y ==> (y DIV 2 = (y-1) DIV 2)`,
+  simp[ODD_EXISTS, PULL_EXISTS, ADD1, ADD_DIV_RWT]);
 
 val WRITE_0_HEAD_lem = Q.store_thm("WRITE_0_HEAD_lem",
-`∀ tm s. (UPDATE_ACT_S_TM s Wr0 tm).tape_h = Z`,
-rpt strip_tac >> rw[UPDATE_ACT_S_TM_def] );
+  `∀ tm s. (UPDATE_ACT_S_TM s Wr0 tm).tape_h = Z`,
+  rpt strip_tac >> rw[UPDATE_ACT_S_TM_def] );
 
 
 val WRITE_1_HEAD_lem = Q.store_thm("WRITE_1_HEAD_lem",
-`∀ tm s. (UPDATE_ACT_S_TM s Wr1 tm).tape_h = O`,
-rpt strip_tac >> rw[UPDATE_ACT_S_TM_def] );
+  `∀ tm s. (UPDATE_ACT_S_TM s Wr1 tm).tape_h = O`,
+  rpt strip_tac >> rw[UPDATE_ACT_S_TM_def] );
 
 val ODD_TL_DECODE_lem = Q.store_thm ("ODD_TL_DECODE_lem",
-`∀ n. (ODD n) ==> (TL (DECODE n) = DECODE ((n-1) DIV 2))`,
-rpt strip_tac >> `EVEN 0` by EVAL_TAC >> `~(n = 0)` by metis_tac[EVEN_AND_ODD]>>
-rw[DECODE_def] >> Cases_on `DECODE n` >- `n=0` by fs[DECODE_EMPTY_lem] >>
-EVAL_TAC >> Cases_on `n` >- fs[] >> fs[DECODE_def] >> rfs[] );
-
+  `∀ n. ODD n ==> (TL (DECODE n) = DECODE ((n-1) DIV 2))`,
+  rpt strip_tac >> `EVEN 0` by EVAL_TAC >> `n ≠ 0` by metis_tac[EVEN_AND_ODD]>>
+  rw[DECODE_def] >> Cases_on `DECODE n` >- `n=0` by fs[DECODE_EMPTY_lem] >>
+  EVAL_TAC >> Cases_on `n` >- fs[] >> fs[DECODE_def] >> rfs[] );
 
 val EVEN_TL_DECODE_lem = Q.store_thm ("EVEN_TL_DECODE_lem",
-`∀ n. ((EVEN n) ∧ (n > 0)) ==> (TL (DECODE n) = DECODE (n DIV 2))`,
-rpt strip_tac >> Cases_on `n` >- fs[]  >>
-    rw[DECODE_def] >> metis_tac[EVEN_AND_ODD] );
-
-
-val EVEN_ENCODE_Z_DECODE_lem = Q.store_thm ("EVEN_ENCODE_Z_DECODE_lem",
-`∀ n. (EVEN n) ==> (n = ENCODE (Z::DECODE (n DIV 2)))`,
-rpt strip_tac >> Cases_on `n` >- EVAL_TAC >> rfs[DECODE_def,ENCODE_def] >>
- rw[ENCODE_DECODE_thm] >> `(SUC n') MOD 2 = 0` by metis_tac[EVEN_MOD2] >>
-`2*(SUC n' DIV 2) = SUC n'` by fs[MULT_EQ_DIV] >> rw[] );
-
-val ODD_ENCODE_O_DECODE_lem = Q.store_thm ("EVEN_ENCODE_Z_DECODE_lem",
-`∀ n. (ODD n) ==> (n = ENCODE (O::DECODE ((n-1) DIV 2)))`,
-rpt strip_tac >> Cases_on `n` >- fs[] >> rfs[DECODE_def,ENCODE_def] >>
-    rw[ENCODE_DECODE_thm] >> `~(ODD n')` by fs[ODD] >> `EVEN n'` by metis_tac[EVEN_OR_ODD] >>
-`n' MOD 2 = 0` by metis_tac[EVEN_MOD2] >>
-`2*( n' DIV 2) =  n'` by fs[MULT_EQ_DIV] >> rw[] );
-
-
-val ODD_MINUS_1_lem = Q.store_thm ("ODD_MINUS_1_lem",
-`∀ n. (ODD n) ==> (~ODD (n-1))`,
-rpt strip_tac >> Cases_on `n` >- fs[] >> `SUC n' - 1 = n'` by fs[SUC_SUB1] >>
-`ODD n'` by fs[] >> fs[ODD] )
-
-
-val ONE_LE_ODD_lem = Q.store_thm ("ONE_LE_ODD_lem",
-`∀n. (ODD n) ==> (1 <= n)`,
-rpt strip_tac >> Cases_on `n` >-  fs[] >> `SUC n' = 1+n'` by fs[SUC_ONE_ADD] >>
-rw[])
-
+  `∀ n. ((EVEN n) ∧ (n > 0)) ==> (TL (DECODE n) = DECODE (n DIV 2))`,
+  rpt strip_tac >> Cases_on `n` >- fs[]  >>
+  rw[DECODE_def] >> metis_tac[EVEN_AND_ODD] );
 
 val ODD_MOD_TWO_lem = Q.store_thm ("ODD_MOD_TWO_lem",
-`∀n. (ODD n) ==> (n MOD 2 = 1)`,
-rpt strip_tac  >> fs[MOD_2] >> `~(EVEN n)` by metis_tac[EVEN_AND_ODD] >> rw[] );
-
-
-val oleast_eq_none = Q.store_thm("oleast_eq_none",
-`($OLEAST P = NONE) <=> (∀n. ¬(P n)) `,
-DEEP_INTRO_TAC whileTheory.OLEAST_INTRO >> simp[] >> metis_tac[]);
+  `∀n. (ODD n) ==> (n MOD 2 = 1)`,
+  rpt strip_tac  >> fs[MOD_2] >> `~EVEN n` by metis_tac[EVEN_AND_ODD] >> rw[]);
 
 val containment_lem = Q.store_thm("containment_lem",
 `((OLEAST n. (NUM_TO_STATE (nfst n),CELL_NUM (nsnd n)) ∈ FDOM p) =
   NONE) <=> (p = FEMPTY)`,
-rw[oleast_eq_none] >> eq_tac >> simp[] >> csimp[fmap_EXT] >>
+rw[] >> eq_tac >> simp[] >> csimp[fmap_EXT] >>
 simp[EXTENSION,pairTheory.FORALL_PROD,NUM_TO_STATE_def] >> strip_tac >>
 qx_gen_tac `a` >> qx_gen_tac `b` >>
 `∃n. a= <| n := n|>  ` by metis_tac[theorem"state_literal_nchotomy"] >>
@@ -603,65 +358,31 @@ val SND_SND_DECODE_TM_TAPE = Q.store_thm("SND_SND_DECODE_TM_TAPE",
 rw[DECODE_TM_TAPE_def] >> `ODD (nsnd (nsnd tmn))` by metis_tac[EVEN_OR_ODD] >>
   rw[ODD_DIV_2_lem]);
 
-
-
-val FST_SND_DECODE_TM_TAPE = Q.store_thm("FST_SND_DECODE_TM_TAPE",
-`ODD (nsnd (nsnd tmn)) ==> (FST (SND (DECODE_TM_TAPE (nsnd tmn))) = O)`,
-rw[DECODE_TM_TAPE_def] >> metis_tac[EVEN_AND_ODD]);
-
-val FST_SND_DECODE_TM_TAPE_EVEN = Q.store_thm("FST_SND_DECODE_TM_TAPE",
-`EVEN (nsnd (nsnd tmn)) ==> (FST (SND (DECODE_TM_TAPE (nsnd tmn))) = Z)`,
-rw[DECODE_TM_TAPE_def]);
-
-
-
-val SND_SND_DECODE_TM_TAPE_FULL = Q.store_thm("SND_SND_DECODE_TM_TAPE_FULL[simp]",
-`SND (SND (DECODE_TM_TAPE (t))) = DECODE (nsnd ( t) DIV 2)`,
-rw[DECODE_TM_TAPE_def] >> `ODD (nsnd (t))` by metis_tac[EVEN_OR_ODD] >>
+val SND_SND_DECODE_TM_TAPE_FULL = Q.store_thm(
+  "SND_SND_DECODE_TM_TAPE_FULL[simp]",
+  `SND (SND (DECODE_TM_TAPE (t))) = DECODE (nsnd ( t) DIV 2)`,
+  rw[DECODE_TM_TAPE_def] >> `ODD (nsnd (t))` by metis_tac[EVEN_OR_ODD] >>
   rw[ODD_DIV_2_lem]);
 
-val FST_SND_DECODE_TM_TAPE_FULL = Q.store_thm("FST_SND_DECODE_TM_TAPE_FULL[simp]",
-`ODD (nsnd (t)) ==> (FST (SND (DECODE_TM_TAPE (t))) = O)`,
-rw[DECODE_TM_TAPE_def] >> metis_tac[EVEN_AND_ODD]);
+val FST_SND_DECODE_TM_TAPE_FULL = Q.store_thm(
+  "FST_SND_DECODE_TM_TAPE_FULL[simp]",
+  `ODD (nsnd (t)) ==> (FST (SND (DECODE_TM_TAPE (t))) = O)`,
+  rw[DECODE_TM_TAPE_def] >> metis_tac[EVEN_AND_ODD]);
 
-val FST_SND_DECODE_TM_TAPE_EVEN_FULL = Q.store_thm("FST_SND_DECODE_TM_TAPE_FULL[simp]",
-`EVEN (nsnd (t)) ==> (FST (SND (DECODE_TM_TAPE (t))) = Z)`,
-rw[DECODE_TM_TAPE_def]);
-
-val OLEAST_EQ_SOME = Q.store_thm(
-"OLEAST_EQ_SOME",
-`($OLEAST P = SOME n) ⇔ P n ∧ ∀m. m < n ⇒ ¬P m`,
-DEEP_INTRO_TAC whileTheory.OLEAST_INTRO >> simp[] >> rpt strip_tac >> EQ_TAC
- >- (rw[] >> rw[]) >- (strip_tac >> metis_tac [DECIDE ``(n':num < n) ∨ (n' = n) ∨ (n < n')``]))
+val FST_SND_DECODE_TM_TAPE_EVEN_FULL = Q.store_thm(
+  "FST_SND_DECODE_TM_TAPE_FULL[simp]",
+  `EVEN (nsnd (t)) ==> (FST (SND (DECODE_TM_TAPE (t))) = Z)`,
+  rw[DECODE_TM_TAPE_def]);
 
 val MEMBER_CARD = Q.store_thm(
-"MEMBER_CARD",
-`a ∈ FDOM p ⇒ 0 < CARD (FDOM p)`,
-Induct_on `p` >> simp[] )
-
-val nfst_lem = Q.store_thm("nfst_lem",
-`(∀n. P (nfst n)) ==> (∀k. P k)`,
-strip_tac >> Induct_on `k` >- (`nfst 0 = 0` by EVAL_TAC >> `P (nfst 0)` by fs[]>> metis_tac[] )
-          >- (`∃l j. nfst (l *, j)= SUC k` by fs[nfst_npair] >>
-`P (nfst (l *, j)) ` by rfs[]  >>  metis_tac[]  ) );
-
-val nsnd_lem = Q.store_thm("nfst_lem",
-`(∀n. P (nsnd n)) ==> (∀k. P k)`,
-strip_tac >> Induct_on `k` >- (`nsnd 0 = 0` by EVAL_TAC >> `P (nsnd 0)` by fs[]>> metis_tac[] )
-          >- (`∃l j. nsnd (l *, j)= SUC k` by fs[nsnd_npair] >>
-`P (nsnd (l *, j)) ` by rfs[]  >>  metis_tac[]  ) );
-
-val nfst_nsnd_lem = Q.store_thm("nfst_nsnd_lem",
-`(∀n. P (nfst n) (nsnd n)) <=> (∀k j. P j k)`,
-eq_tac >> simp[] >>
-rpt strip_tac >> ` nsnd (j *, k)=  k` by fs[nsnd_npair] >> ` nfst (j *, k)= j` by fs[nfst_npair] >> `P (nfst (j *, k)) (nsnd (j *, k)) ` by fs[] >> metis_tac[] );
+  "MEMBER_CARD",
+  `a ∈ FDOM p ⇒ 0 < CARD (FDOM p)`,
+  Induct_on `p` >> simp[] );
 
 val npair_lem = Q.store_thm("npair_lem",
-`(∀n. P n) <=> (∀j k. P (j *, k))`,
-eq_tac >> simp[] >>
-rpt strip_tac >> `∃j k. j *, k = n` by metis_tac[npair_cases] >> rw[] );
-
-
+  `(∀n. P n) <=> (∀j k. P (j *, k))`,
+  eq_tac >> simp[] >>
+  rpt strip_tac >> `∃j k. j *, k = n` by metis_tac[npair_cases] >> rw[] );
 
 val NUM_TO_CELL_TO_NUM = Q.store_thm("NUM_TO_CELL_TO_NUM",
 `((c=0) ∨ (c=1)) ==> (NUM_CELL (CELL_NUM c) = c)`,
@@ -701,8 +422,8 @@ strip_tac >> `tm.prog = tm'.prog` by simp[] >> rw[] >>
 ` FDOM tm.prog DELETE (a,b) = FDOM tm.prog` by  metis_tac[] >>  simp[DELETE_NON_ELEMENT] )
 
 val TM_ACT_LEM_1 = Q.store_thm("TM_ACT_LEM_1[simp]",
-`( (nsnd (nsnd (FULL_ENCODE_TM tm))) MOD 2) = NUM_CELL (tm.tape_h)`,
-simp[FULL_ENCODE_TM_def,ENCODE_TM_TAPE_def] >> rw[] >> Cases_on `tm.tape_h` >- fs[] >- EVAL_TAC)
+  `( (nsnd (nsnd (FULL_ENCODE_TM tm))) MOD 2) = NUM_CELL (tm.tape_h)`,
+  simp[FULL_ENCODE_TM_def,ENCODE_TM_TAPE_def] >> rw[] >> Cases_on `tm.tape_h` >- fs[] >- EVAL_TAC)
 
 val _ = add_rule {term_name = "FULL_ENCODE_TM",fixity = Closefix, block_style = (AroundEachPhrase,(PP.CONSISTENT,0)),paren_style = OnlyIfNecessary,pp_elements = [TOK "⟦",TM,TOK"⟧"]}
 
